implement wojciech idea

LeanSAT/Model/Quantifiers.lean
@@ -3,11 +3,11 @@
 Authors: James Gallicchio
 -/
 
-import LeanSAT.Model.Subst
+import LeanSAT.Model.OfFun
 
 namespace LeanSAT.Model
 
-/-! ## Existential Quantifiers
+/-! ## Quantification
 
 The main result of this file is a characterization of
 existential quantification over [PropFun].
@@ -17,316 +17,63 @@ Quantifying over a single variable is straightforward
 Quantifying over a *set* of variables is less straightforward.
 -/
 
-/-! ### Single Variable -/
-
-namespace PropForm
-
-def existQuant [DecidableEq ν] (φ : PropForm ν) (v : ν) : PropForm ν :=
-  disj (φ.substOne v .fls)
-       (φ.substOne v .tr)
-
-theorem satisfies_existQuant [DecidableEq ν] (φ : PropForm ν) (v : ν) {τ : PropAssignment ν}
-  : τ ⊨ φ.existQuant v ↔ τ ⊨ φ.substOne v .fls ∨ τ ⊨ φ.substOne v .tr
-  := by simp [existQuant]
-
-end PropForm
-
 namespace PropFun
 
-variable [DecidableEq ν] (φ : PropFun ν) (v : ν)
+variable [DecidableEq ν] [DecidableEq ν'] [Fintype ν] [Fintype ν']
 
-def existQuant : PropFun ν :=
-    (φ.substOne v ⊥)
-  ⊔ (φ.substOne v ⊤)
-
-theorem satisfies_existQuant (τ : PropAssignment ν)
-  : τ ⊨ φ.existQuant v ↔ ∃ b, τ.set v b ⊨ φ := by
-  simp [existQuant, satisfies_substOne]
-
-theorem existQuant_comm (v₁ v₂ : ν)
-  : (φ.existQuant v₁ |>.existQuant v₂) = (φ.existQuant v₂ |>.existQuant v₁)
-  := by
-  if h' : v₁ = v₂ then
-    cases h'; rfl
-  else
-  ext τ
-  simp [existQuant, satisfies_disj, satisfies_substOne]
-  generalize eval τ ⊤ = _τ1
-  generalize eval τ ⊥ = _τ2
-  -- TODO: rewrite this to be a terminal aesop call
-  aesop <;> (
-    rw [PropAssignment.set_comm] at h
-    simp [h]
-    first | exact h' | exact ne_comm.mp h')
-
-theorem semVars_existQuant : semVars (φ.existQuant v) ⊆ semVars φ \ {v} := by
-  intro v'
-  simp [mem_semVars, existQuant, satisfies_substOne]
-  push_neg
-  rintro τ h1 ⟨h2,h3⟩
-  if h:v = v' then
-    cases h
-    simp_all
-  else
-    simp [Ne.symm h]
-    rw [PropAssignment.set_comm] at h2 h3
-    · rcases h1 with h1|h1
-        <;> (
-        refine ⟨_,h1,?_⟩
-        rw [PropAssignment.set_get_of_ne]
-        repeat assumption)
-    repeat assumption
-
-theorem existQuant_eq_of_not_mem_semVars
-  : ¬v ∈ φ.semVars → existQuant φ v = φ := by
-  intro h
-  ext τ
-  simp [satisfies_existQuant]
-  convert @or_self_iff (τ ⊨ φ) using 2 <;> (
-    apply PropFun.agreeOn_semVars
-    apply PropAssignment.agreeOn_set_of_not_mem
-    apply h
-  )
-
-@[simp] theorem existQuant_top : existQuant ⊤ v = ⊤ := by
-  ext τ
-  simp [satisfies_existQuant]
-
-
-/-! ### Sets of Variables -/
-
-def existQuantSet (φ : PropFun ν) [DecidableEq ν] (vs : Finset ν) : PropFun ν :=
-  vs.elim (fun L _ => L.foldl existQuant φ) pf
-where
-  pf := by
-    intro a b ha hb
-    have h1 := ha
-    rw [←hb] at h1
-    have : a ~ b := Quotient.eq_rel.mp h1
-    simp; clear ha hb h1
-    induction this generalizing φ with
-    | nil         => simp at *
-    | cons _ _ ih => simp at *; apply ih
-    | swap        => simp; rw [existQuant_comm]
-    | trans _ _ ih1 ih2 =>
-      rw [ih1, ih2]
-
-theorem satisfies_existQuantSet (φ : PropFun ν) [DecidableEq ν] (vs : Finset ν) (τ : PropAssignment ν)
-  : τ ⊨ φ.existQuantSet vs ↔ ∃ τ', τ.setMany vs τ' ⊨ φ := by
-  simp [existQuantSet]
-  apply Finset.elim_eq_forall (s := vs)
-    (f := fun L _ => List.foldl existQuant φ L)
-    (h := existQuantSet.pf _ _)
-  intro L hL hs
-  rcases vs with ⟨vs,h⟩
-  cases hL
-  rw [hs]; clear hs
-  unfold PropAssignment.setMany; simp; clear h
-  induction L generalizing φ with
-  | nil =>
-    simp [PropAssignment.setMany]
-  | cons x xs ih =>
-    simp
-    rw [ih]; clear ih
-    simp only [satisfies_existQuant]
-    constructor
-    · rintro ⟨τ', b, h⟩; refine ⟨τ'.set x b, ?_⟩
-      convert h using 1; ext v
-      simp [PropAssignment.set]
-      aesop
-    · rintro ⟨τ', h⟩; refine ⟨τ', τ' x, ?_⟩
-      convert h using 1; ext v
-      simp [PropAssignment.set]
-      aesop
-
-def semVars_existQuantSet (φ : PropFun ν) [DecidableEq ν] (vs : Finset ν)
-  : semVars (φ.existQuantSet vs) ⊆ φ.semVars \ vs := by
-  rcases vs with ⟨vs,h⟩
-  have ⟨L,h⟩ := Quotient.exists_rep vs; cases h
-  simp [existQuantSet, Finset.elim]
-  rw [Multiset.elim_mk]
-  induction L generalizing φ with
-  | nil => simp
-  | cons hd tl ih =>
-    simp at h; simp_all
-    intro v hv
-    have := ih _ hv
-    simp at this
-    rcases this with ⟨hhd,htl⟩
-    have := semVars_existQuant φ hd hhd
-    simp at this
-    simp [*]
-
-theorem existQuantSet_eq_of_semVars_disjoint
-  : Disjoint (φ.semVars) vs → existQuantSet φ vs = φ
-  := by
-  intro hdis
-  ext τ
-  simp [satisfies_existQuantSet]
-  have : ∀ τ', (τ.setMany vs τ').agreeOn φ.semVars τ := by
-    intro τ'
-    apply PropAssignment.agreeOn_setMany_of_disjoint
-    simp [hdis]
-  simp [PropFun.agreeOn_semVars (this _)]
-
-theorem existQuantSet_existQuantSet (φ : PropFun ν) (vs vs' : Finset ν)
-  : (φ.existQuantSet vs).existQuantSet vs' = φ.existQuantSet (vs' ∪ vs)
-  := by
-  ext τ
-  simp [satisfies_existQuantSet, PropAssignment.setMany_setMany]
-  constructor
-  · rintro ⟨τ1,τ2,h⟩
-    exact ⟨_,h⟩
-  · rintro ⟨τ1,h⟩
-    refine ⟨τ1,τ1,?_⟩
-    simp [h]
-
-theorem existQuantSet_union_of_disjoint_semVars_right (φ : PropFun ν) (vs vs' : Finset ν)
-  : Disjoint φ.semVars vs' → φ.existQuantSet (vs ∪ vs') = φ.existQuantSet vs := by
-  intro h; rw [← existQuantSet_existQuantSet, existQuantSet_eq_of_semVars_disjoint _ h]
-
-theorem existQuantSet_eq_of_inter_semVars_eq (φ : PropFun ν) (vs vs' : Finset ν)
-  : vs ∩ φ.semVars = vs' ∩ φ.semVars → φ.existQuantSet vs = φ.existQuantSet vs' := by
-  intro h
-  ext τ; simp [satisfies_existQuantSet]
-  conv => lhs; arg 1; ext; rw [PropFun.setMany_satisfies_iff_inter_semVars, h]
-  conv => rhs; arg 1; ext; rw [PropFun.setMany_satisfies_iff_inter_semVars]
-
-@[simp] theorem existQuantSet_top [DecidableEq ν] (vs : Finset ν)
-  : existQuantSet ⊤ vs = ⊤ := by
-  ext τ
-  simp [satisfies_existQuantSet]
-
-theorem existQuantSet_conj [DecidableEq ν] (a b : PropFun ν) (vs)
-  : Disjoint b.semVars vs → existQuantSet (a ⊓ b) vs = existQuantSet a vs ⊓ b
-  := by
-  intro h
-  ext τ
-  have := fun τ' =>
-    PropAssignment.agreeOn_setMany_of_disjoint
-      τ (semVars b) vs τ' (by simp; exact h)
-  simp [satisfies_existQuantSet, PropFun.agreeOn_semVars (this _)]
-
-/-
-theorem existQuantSet_pmap [DecidableEq ν'] [Fintype ν] (f : φ.semVars → ν') (vs : Finset ν')
-  : existQuantSet (pmap φ f) vs =
-      pmap (existQuantSet φ (Finset.univ.filter (fun v =>
-          if h : _ then f ⟨v,h⟩ ∈ vs else false))) (fun ⟨v,h⟩ =>
-              f ⟨v, by have := semVars_existQuantSet _ _ h; simp at this; simp [*]⟩) := by
-  ext τ
-  stop
-  simp [satisfies_existQuantSet, satisfies_invImage]
-  constructor
-  · rintro ⟨τ', hsat⟩
-    use (fun v =>
-      if h : v ∈ vs.map f then
-        τ' ((Finset.mapEquiv vs f).symm ⟨v,h⟩)
-      else
-        false)
-    refine (agreeOn_semVars ?_).mp hsat
-    · intro v hv
-      simp [invImage.assn, PropAssignment.setMany]
-      aesop
-  · rintro ⟨τ', hsat⟩
-    use (fun v' =>
-      if v' ∈ vs then
-        τ' (f v')
-      else
-        false)
-    refine (agreeOn_semVars ?_).mp hsat
-    · intro v hv
-      simp [invImage.assn, PropAssignment.setMany]
-      have : ∀ w, w ∈ vs' → w ∈ vs := h
-      aesop
+/-- Most general form of existential quantification.
+True at `τ` iff there exists a model of `φ` whose image under `f` is `τ`.
 -/
+def «exists» (f : PropAssignment ν → PropAssignment ν') (φ : PropFun ν) : PropFun ν' :=
+  ofSet { τ | ∃ σ, σ ⊨ φ ∧ τ = f σ }
 
-noncomputable def existQuantInv [DecidableEq ν'] (f : ν ↪ ν') [Fintype ν] (φ : PropFun ν') : PropFun ν :=
-  φ |>.existQuantSet (φ.semVars \ Finset.univ.map f)
-    |>.preimage f
+@[simp]
+theorem satisfies_exists {A B C D} (f : PropAssignment ν → PropAssignment ν') (τ)
+  : τ ⊨ @«exists» ν ν' A B C D f φ ↔ ∃ σ, σ ⊨ φ ∧ τ = f σ := by
+  simp [«exists»]
 
-theorem existQuantInv_conj [DecidableEq ν'] (f : ν ↪ ν') [Fintype ν]
-  : existQuantInv f (φ₁ ⊓ φ₂.map f) = existQuantInv f φ₁ ⊓ φ₂ := by
-  simp [existQuantInv]
-  rw [existQuantSet_conj _ _ _ ?disj]
-  case disj =>
-    apply Finset.disjoint_of_subset_left (u := Finset.univ.map f)
-    · intro v' hv'
-      rw [semVars_map] at hv'
-      simp at hv' ⊢; rcases hv' with ⟨v,hv,h⟩; use v; apply h
-    · apply Finset.disjoint_sdiff
-  rw [existQuantSet_eq_of_inter_semVars_eq (vs' := semVars φ₁ \ Finset.univ.map f)]
-  · rw [preimage_conj _ _ _ ?hp ?hq]
-    case hp =>
-      trans; apply semVars_existQuantSet
-      simp; apply Finset.inter_subset_right
-    case hq =>
-      rw [semVars_map]
-      repeat sorry
-    simp
-  · sorry
-  stop
-  unfold existQuantInv
-  suffices ∀ φ h, φ = existQuantSet _ _ → invImage f Finset.univ φ h = _
-    from this _ _ rfl
-  intro φ h hφ
-  ext τ; simp [satisfies_invImage]
-  generalize hA : φ₁.semVars = A
-  generalize hB : Finset.univ.map f = B at hφ
-  generalize hC : (φ₂.map f).semVars = C
-  generalize hD : (φ₁ ⊓ φ₂.map f).semVars = D at hφ
-  have cb : C ⊆ B := by rw [←hC, ←hB]; apply _root_.trans; apply semVars_map; intro x; aesop
-  have dac : D ⊆ A ∪ C := by rw [←hA,←hC,←hD]; apply semVars_conj _ _
-  have dba : D \ B ⊆ A \ B := by
-    clear hφ; intro x
-    replace cb := @cb x
-    replace dac := @dac x
-    intro h
-    simp at *
-    aesop
-  have : Disjoint D ((A \ B) \ (D \ B)) := by
-    rw [Finset.disjoint_iff_ne]
-    intro x hx y hy
-    aesop
-  conv at this => arg 1; rw [← hD]
-  rw [← existQuantSet_union_of_disjoint_semVars_right _ _ _ this] at hφ
-  clear this
-  rw [PropFun.existQuantSet_conj] at hφ
-  · cases hφ; simp; intro
-    apply iff_of_eq; congr
-    exact Finset.union_eq_right.mpr dba
-  · rw [hC]; simp
-    constructor <;> (apply Finset.disjoint_of_subset_left cb; apply Finset.disjoint_sdiff)
+def existsInv (f : ν' → ν) (φ : PropFun ν): PropFun ν' :=
+  φ.exists (fun σ => σ.map f)
 
-set_option pp.proofs.withType false
-theorem existQuantInv_existQuantInv
-    [DecidableEq ν] [DecidableEq ν'] [DecidableEq ν'']
-    [Fintype ν] [Fintype ν'] [Fintype ν'']
-    (f : ν'' ↪ ν') (g : ν' ↪ ν)
-  : existQuantInv f (existQuantInv g φ) = existQuantInv (f.trans g) φ := by
-  ext τ
-  unfold Function.Embedding.trans
-  simp [existQuantInv]
-  conv => lhs; rw [satisfies_preimage]
-  conv => rhs; rw [satisfies_preimage]
-  rw [existQuantSet_invImage, satisfies_invImage]
-  · rw [existQuantSet_existQuantSet]
-    apply iff_of_eq; congr 1
-    · sorry
-    · congr 1
-      ext v; simp
-      constructor
-      · rintro (⟨v',⟨h1,h2⟩,rfl⟩|⟨h1,h2⟩)
-        · have := semVars_invImage_subset_preimage _ _ _ _ h1
-          simp at this
-          have := semVars_existQuantSet _ _ this
-          simp at this; simp [this]
-          intro v''; apply h2
-        · simp [h1, h2]
-      · rintro ⟨h1,h2⟩
-        simp [h1]
-        rw [Classical.or_iff_not_imp_right]
-        simp; intro x hx; use x; simp [*]
-        constructor
-        · apply semVars_invImage_subset_preimage; sorry
-        · intro v''; have := h2 v''; cases hx; simp at this; use this
-  · intro; simp
+@[simp]
+theorem satisfies_existsInv {A B C D} (f : ν' → ν) (φ) (τ)
+  : τ ⊨ @«existsInv» ν ν' A B C D f φ ↔ ∃ σ : PropAssignment ν, σ ⊨ φ ∧ τ = σ.map f := by
+  simp [«existsInv»]
+
+@[simp]
+theorem existsInv_existsInv [DecidableEq ν''] [Fintype ν'']
+      (f : ν'' → ν') (g : ν' → ν) (φ : PropFun ν)
+  : (φ.existsInv g).existsInv f = φ.existsInv (g ∘ f) := by
+  ext τ; simp
+  constructor
+  · rintro ⟨_, ⟨σ,h,rfl⟩, rfl⟩
+    use σ
+    simp [*, PropAssignment.map]
+    rfl
+  · rintro ⟨σ,h,rfl⟩
+    use σ.map g
+    simp [*, PropAssignment.map, Function.comp]
+    use σ
+
+
+/-- Most general form of universal quantification.
+True at `τ` iff for all models of `φ`, their image under `f` is `τ`.
+-/
+def «forall» (f : PropAssignment ν → PropAssignment ν') (φ : PropFun ν) : PropFun ν' :=
+  ofSet { σ | ∀ τ, τ ⊨ φ → σ = f τ }
+
+@[simp]
+theorem satisfies_forall (f : PropAssignment ν → PropAssignment ν') (τ)
+  : τ ⊨ «forall» f φ ↔ ∀ σ, σ ⊨ φ → τ = f σ := by
+  simp [«forall»]
+
+def forallInv (f : ν' → ν) (φ : PropFun ν): PropFun ν' :=
+  φ.forall (fun σ => σ.map f)
+
+@[simp]
+theorem satisfies_forallInv (f : ν' → ν) (φ) (τ)
+  : τ ⊨ «forallInv» f φ ↔ ∀ σ : PropAssignment ν, σ ⊨ φ → τ = σ.map f := by
+  simp [«forallInv»]
+
+
+end PropFun
